Map literal improvements and Unit test (#323)
This accompanies goose PR
[#122](https://github.com/goose-lang/goose/pull/122).

I've been working on improving support for map literal, and now have a
complete unit test for creating and returning one. This proved to be
more complex than I originally suspected since the key-value pairs in
the list expressions output by goose cannot be evaluated to values with
the previous automated tactics. The work here introduces a new `IntoVal`
instance for tuples, but doesn't provide any `PureWp` rules for it to
prevent any conflicts with struct fields or other places were tuples of
values are used. Instead, map literals are now generated using a wrapper
called `map.kv_entry` which can be evaluated into a value with tactics
like `wp_auto`.

new/golang/defn/map.v
@@ -69,6 +69,12 @@ Definition len : val :=
 Definition make : val :=
   λ: "kt" "vt", Alloc (InjL (type.zero_val "vt")).
 
+Definition kv_entry_def : val :=
+  λ: "k" "v", ("k", "v").
+Program Definition kv_entry := unseal (_:seal (@kv_entry_def)).
+Obligation 1. by eexists. Qed.
+Definition kv_entry_unseal : @kv_entry = _ := seal_eq _.
+
 Definition literal_val : val :=
   rec: "lit_val" "kt" "vt" "alist" :=
     list.Match "alist"
