new/golang/theory/map.v
@@ -50,17 +50,27 @@ Context `{!IntoValTyped K kt} `{!IntoValTyped V vt}.
 Notation "mref ↦$ dq m" := (own_map mref dq m)
                             (at level 20, dq custom dfrac at level 50, format "mref  ↦$ dq  m").
 
-Lemma wp_map_literal_val (l:list (K * V)) (v:val):
-  {{{ ⌜ v = map_list_val l ⌝ }}}
-    map.literal_val #kt #vt v
+Global Instance wp_kv_entry_pure_wp {A B:Type} `{!IntoVal A} `{!IntoVal B} (a: A) (b: B) :
+  PureWp True ((map.kv_entry #a #b)%E) (#(a, b)).
+Proof.
+  pure_wp_start.
+  rewrite map.kv_entry_unseal.
+  unfold map.kv_entry_def.
+  wp_pure_lc "?".
+  wp_pures.
+  rewrite [in #(_, _)]to_val_unseal /=.
+  iApply "HΦ".
+  done.
+Qed.
+
+Lemma wp_map_literal_val (l:list (K * V)):
+  {{{ True }}}
+    map.literal_val #kt #vt #l
   {{{ v, RET v; ⌜ is_map_val v (list_to_map l) ⌝ }}}.
 Proof. 
-  iIntros (?) "% HΦ". subst.
+  iIntros (?) "% HΦ".
   iInduction l as [| h tl] "IH" forall (Φ).
   + wp_call.
-    rewrite map_list_val_unseal /=.
-    rewrite list.Match_unseal /=.
-    wp_call_lc "?".
     iApply "HΦ".
     iPureIntro.
     unfold is_map_val. 
@@ -68,17 +78,16 @@ Proof.
     - done.
     - symmetry. apply default_val_eq_zero_val.
   + wp_call.
-    rewrite map_list_val_unseal /=.
-    rewrite list.Match_unseal /=.
-    wp_call_lc "?".
     wp_bind (map.literal_val _ _ _)%E. 
     iApply ("IH" with "[HΦ]"). iNext.
     iIntros (?) "%Htl_map".
     wp_pures.
     iApply "HΦ".
     iPureIntro.
-    unfold is_map_val.
-    exists (fst h), (snd h), (list_to_map tl).
+    destruct h as [hk hv].
+    rewrite to_val_unseal.
+    simpl.
+    exists hk, hv, (list_to_map tl).
     split; first reflexivity.
     split; first reflexivity.
     split.
@@ -88,14 +97,14 @@ Proof.
     - reflexivity.
 Qed. 
      
-Lemma wp_map_literal (l:list (K * V)) (v:val):
-  {{{ ⌜ v = map_list_val l ⌝ ∗ ⌜ is_comparable_go_type kt = true ⌝ }}}
-    map.literal #kt #vt v
+Lemma wp_map_literal (l:list (K * V)):
+  {{{ ⌜ is_comparable_go_type kt = true ⌝ }}}
+    map.literal #kt #vt #l
   {{{ (l_ptr : loc), RET #l_ptr; l_ptr ↦$ (list_to_map l) }}}.
 Proof.
-  iIntros (?) "[%Hlst %Hcomp] HΦ". subst.
+  iIntros (?) "%Hcomp HΦ".
   wp_call.
-  wp_apply wp_map_literal_val; first done.
+  wp_apply wp_map_literal_val.
   iIntros (v) "%Hmv".
   iApply (wp_alloc_untyped with "[//]").
   { instantiate (1:=v). by destruct v. }
